Implement a decision algorithm for nesting

LambdaGraph/Algorithms.lean
@@ -175,37 +175,55 @@ instance {e : Expr} {q : Nat → RefKind → Prop} [DecidableRel q] :
 instance {e : Expr} {n : Nat} : Decidable (e.Bounded n) :=
   inferInstanceAs (Decidable (∀ m r, e.Local m r → m < n))
 
-inductive Path (p : Program) : Nat → Nat → Type where
-  | refl n : n < p.size → Path p n n
-  | step m n k : m ⟶[p] n → Path p n k → Path p m k
+abbrev Rel : Type := Nat → Nat → Prop
 
-def Path.length {p : Program} {m n : Nat} : Path p m n → Nat
-  | refl _ _ => 0
+inductive Path (r : Rel) : Nat → Nat → Type where
+  | refl n : Path r n n
+  | step m n k : r m n → Path r n k → Path r m k
+
+def Path.length {r : Rel} {m n : Nat} : Path r m n → Nat
+  | refl _ => 0
   | step _ _ _ _ path => path.length + 1
 
-def Path.labels {p : Program} {m n : Nat} : Path p m n → Finset
-  | refl n _ => {n}
+def Path.labels {r : Rel} {m n : Nat} : Path r m n → Finset
+  | refl n => {n}
   | step n _ _ _ path => path.labels.insert n
 
-inductive Path.Mem {p : Program} (l : Nat) : ∀ {m n}, Path p m n → Prop where
-  | head n (path : Path p l n) : path.Mem l
-  | tail m n k hs (path : Path p n k) : path.Mem l → (path.step m n k hs).Mem l
+inductive Path.Mem {r : Rel} (l : Nat) : ∀ {m n}, Path r m n → Prop where
+  | head n (path : Path r l n) : path.Mem l
+  | tail m n k hs (path : Path r n k) : path.Mem l → (path.step m n k hs).Mem l
 
-instance {p : Program} {m n : Nat} : Membership Nat (Path p m n) where
+instance {r : Rel} {m n : Nat} : Membership Nat (Path r m n) where
   mem path l := path.Mem l
 
 @[simp, grind =]
-theorem Path.length_refl {p : Program} {n : Nat} (hn : n < p.size) :
-    (Path.refl n hn).length = 0 := by simp [length]
-
-@[simp, grind =]
-theorem Path.length_step {p : Program} {m n k : Nat} {path : Path p n k}
-    (h : m ⟶[p] n) : (path.step _ _ _ h).length = path.length + 1 := by
+theorem Path.length_refl {r : Rel} {n : Nat} : (@Path.refl r n).length = 0 := by
   simp [length]
 
 @[simp, grind =]
-theorem Path.mem_refl_iff {p : Program} {l n : Nat} (hn : n < p.size) :
-    l ∈ Path.refl n hn ↔ l = n := by
+theorem Path.length_step {r : Rel} {m n k : Nat} {path : Path r n k}
+    (h : r m n) : (path.step _ _ _ h).length = path.length + 1 := by
+  simp [length]
+
+@[simp, grind =]
+theorem Path.length_eq_zero_iff {r : Rel} {m n : Nat} {path : Path r m n} :
+    path.length = 0 ↔ ∃ (h : m = n), path = h ▸ .refl m := by
+  constructor
+  · intro h
+    cases path with
+    | refl _ => exact ⟨rfl, rfl⟩
+    | step _ k n hs path => simp at h
+  · rintro ⟨rfl, rfl⟩
+    simp
+
+theorem Path.end_mem {r : Rel} {m n : Nat} (path : Path r m n) : n ∈ path :=
+  match path with
+  | refl _ => .head _ _
+  | step _ _ _ _ path => .tail _ _ _ _ _ path.end_mem
+
+@[simp, grind =]
+theorem Path.mem_refl_iff {r : Rel} {l n : Nat} :
+    l ∈ @Path.refl r n ↔ l = n := by
   constructor
   · intro h
     have .head _ _ := h
@@ -214,8 +232,8 @@ theorem Path.mem_refl_iff {p : Program} {l n : Nat} (hn : n < p.size) :
     constructor
 
 @[simp, grind =]
-theorem Path.mem_step_iff {p : Program} {l m n k : Nat} {path : Path p n k}
-    (hs : m ⟶[p] n) : l ∈ path.step _ _ _ hs ↔ l = m ∨ l ∈ path := by
+theorem Path.mem_step_iff {r : Rel} {l m n k : Nat} {path : Path r n k}
+    (hs : r m n) : l ∈ path.step _ _ _ hs ↔ l = m ∨ l ∈ path := by
   constructor
   · intro h
     cases h with
@@ -223,26 +241,14 @@ theorem Path.mem_step_iff {p : Program} {l m n k : Nat} {path : Path p n k}
     | tail _ _ _ _ _ h => exact .inr h
   · rintro (rfl | h) <;> constructor <;> assumption
 
-theorem Path.lt_size_of_mem {p : Program} {l m n : Nat} {path : Path p m n}
-    (h : l ∈ path) : l < p.size := by
-  induction h with
-  | head n path =>
-    cases path with
-    | refl _ hl => exact hl
-    | step _ m _ hs path => exact hs.1
-  | tail m n k hs path h hl => exact hl
+def Path.Bounded {r : Rel} {m k : Nat} (path : Path r m k) (n : Nat) : Prop :=
+  ∀ ⦃l⦄, l ∈ path → l < n
 
-theorem Path.lt_size_right {p : Program} {m n : Nat} (path : Path p m n) :
-    n < p.size := by
-  induction path with
-  | refl n hn => exact hn
-  | step m k n hs path ih => exact ih
-
-theorem Path.labels_correct {p : Program} {l m n : Nat} {path : Path p m n} :
+theorem Path.labels_correct {r : Rel} {l m n : Nat} {path : Path r m n} :
     l ∈ path.labels ↔ l ∈ path := by
   constructor <;> intro h
   · fun_induction labels
-    next n hn =>
+    next n =>
       simp only [Finset.singleton_eq_insert, Finset.mem_insert_iff,
         Finset.notMem_emptyCollection, or_false] at h
       subst n
@@ -254,71 +260,81 @@ theorem Path.labels_correct {p : Program} {l m n : Nat} {path : Path p m n} :
       · apply_rules [Mem.tail]
   · induction h with grind [labels, cases Path]
 
-def Path.push {p : Program} {m n k : Nat} (path : Path p m n) (hk : k < p.size)
-    (h : n ⟶[p] k) : Path p m k :=
+def Path.push {r : Rel} {m n k : Nat} (path : Path r m n) (h : r n k) :
+    Path r m k :=
   match path with
-  | refl _ hm => .step _ _ _ h (.refl _ hk)
-  | step _ _ _ hs path => .step _ _ _ hs (path.push hk h)
+  | refl _ => .step _ _ _ h (.refl _)
+  | step _ _ _ hs path => .step _ _ _ hs (path.push h)
 
 @[simp, grind =]
-theorem Path.length_push {p : Program} {m n k : Nat} {path : Path p m n}
-    (hk : k < p.size) (h : n ⟶[p] k) :
-    (path.push hk h).length = path.length + 1 := by
+theorem Path.length_push {r : Rel} {m n k : Nat} {path : Path r m n}
+    (h : r n k) : (path.push h).length = path.length + 1 := by
   induction path with simp [length, push, *]
 
 @[simp, grind =]
-theorem Path.mem_push_iff {p : Program} {l m n k : Nat} {path : Path p m n}
-    (hk : k < p.size) (h : n ⟶[p] k) :
-    l ∈ path.push hk h ↔ l ∈ path ∨ l = k := by
+theorem Path.mem_push_iff {r : Rel} {l m n k : Nat} {path : Path r m n}
+    (h : r n k) : l ∈ path.push h ↔ l ∈ path ∨ l = k := by
   induction path with grind [push]
 
-theorem Path.split_last {p : Program} {m n : Nat} (path : Path p m n) :
-    (∃ (h : m = n) (hm : m < p.size), path = h ▸ .refl _ hm) ∨
-      ∃ k hk h, ∃ path' : Path p m k, path = path'.push hk h := by
-  induction path with
-  | refl m hm => exact .inl ⟨rfl, hm, rfl⟩
-  | step m k n hs path ih =>
-    obtain ⟨rfl, hm, rfl⟩ | ⟨l, hn, hs', path, rfl⟩ := ih
-    · exact .inr ⟨_, hm, hs, .refl _ hs.1, rfl⟩
-    · exact .inr ⟨_, hn, hs', .step _ _ _ hs path, rfl⟩
+def Path.concat {r : Rel} {m n k : Nat} (path₁ : Path r m n)
+    (path₂ : Path r n k) : Path r m k :=
+  match path₁ with
+  | refl m => path₂
+  | step l m n hs path₁ => .step l m k hs (path₁.concat path₂)
 
-inductive Path.Acyclic {p : Program} : ∀ {m n}, Path p m n → Prop where
-  | refl n hn : (Path.refl n hn).Acyclic
-  | step m n k hs (path : Path p n k) :
+@[simp, grind =]
+theorem Path.length_concat {r : Rel} {m n k : Nat} {path₁ : Path r m n}
+    {path₂ : Path r n k} :
+    (path₁.concat path₂).length = path₁.length + path₂.length := by
+  induction path₁ with simp +arith [concat, *]
+
+theorem Path.split_last {r : Rel} {m n : Nat} (path : Path r m n) :
+    (∃ (h : m = n), path = h ▸ .refl _) ∨
+      ∃ k h, ∃ path' : Path r m k, path = path'.push h := by
+  induction path with
+  | refl m => exact .inl ⟨rfl, rfl⟩
+  | step m k n hs path ih =>
+    obtain ⟨rfl, rfl⟩ | ⟨l, hs', path, rfl⟩ := ih
+    · exact .inr ⟨_, hs, .refl _, rfl⟩
+    · exact .inr ⟨_, hs', .step _ _ _ hs path, rfl⟩
+
+inductive Path.Acyclic {r : Rel} : ∀ {m n}, Path r m n → Prop where
+  | refl n : (Path.refl n).Acyclic
+  | step m n k hs (path : Path r n k) :
     m ∉ path → path.Acyclic → (path.step m n k hs).Acyclic
 
-theorem Path.size_labels_eq_of_acyclic {p : Program} {m n : Nat}
-    {path : Path p m n} (h : path.Acyclic) :
-    path.labels.size = path.length + 1 := by
+theorem Path.size_labels_eq_of_acyclic {r : Rel} {m n : Nat} {path : Path r m n}
+    (h : path.Acyclic) : path.labels.size = path.length + 1 := by
   induction h with
     simp_all! [labels_correct, Finset.size_insert_of_mem,
       Finset.size_insert_of_notMem]
 
-theorem Path.length_lt_size_of_acyclic {p : Program} {m n : Nat}
-    {path : Path p m n} (h : path.Acyclic) : path.length < p.size := by
+theorem Path.length_lt_size_of_acyclic {r : Rel} {n m k : Nat}
+    {path : Path r m k} (h : path.Acyclic) (hb : path.Bounded n) :
+    path.length < n := by
   apply Nat.lt_of_succ_le
   simp only [Nat.succ_eq_add_one, ← size_labels_eq_of_acyclic h]
   apply Finset.size_le_of_all_lt
-  intro k
-  rw [labels_correct]
-  exact lt_size_of_mem
+  intro k hk
+  rw [labels_correct] at hk
+  exact hb hk
 
-theorem Path.exists_of_mem {p : Program} {l m n : Nat} {path : Path p m n}
-    (h : l ∈ path) : ∃ (path' : Path p l n),
+theorem Path.exists_of_mem {r : Rel} {l m n : Nat} {path : Path r m n}
+    (h : l ∈ path) : ∃ (path' : Path r l n),
       path'.length ≤ path.length ∧ ∀ k ∈ path', k ∈ path := by
   induction h with grind
 
-theorem Path.exists_acyclic.aux {p : Program} {b m n : Nat} {path : Path p m n}
-    (hb : path.length ≤ b) : ∃ (path' : Path p m n),
+theorem Path.exists_acyclic.aux {r : Rel} {b m n : Nat} {path : Path r m n}
+    (hb : path.length ≤ b) : ∃ (path' : Path r m n),
       path'.Acyclic ∧ ∀ l ∈ path', l ∈ path := by
   induction b generalizing m n path with
   | zero =>
     cases path with
-    | refl _ hm => exact ⟨.refl m hm, .refl m hm, fun _ h => h⟩
+    | refl _ => exact ⟨.refl m, .refl m, fun _ h => h⟩
     | step _ k n hs path => simp [length] at hb
   | succ b ih =>
     cases path with
-    | refl _ hm => exact ⟨.refl m hm, .refl m hm, fun _ h => h⟩
+    | refl _ => exact ⟨.refl m, .refl m, fun _ h => h⟩
     | step _ k n hs path =>
       simp only [length, Nat.add_le_add_iff_right] at hb
       by_cases hm : m ∈ path
@@ -329,43 +345,99 @@ theorem Path.exists_acyclic.aux {p : Program} {b m n : Nat} {path : Path p m n}
         refine ⟨.step m k n hs path', .step _ _ _ _ _ hm ha, ?_⟩
         grind
 
-theorem Path.exists_acyclic {p : Program} {m n : Nat} (path : Path p m n) :
-    ∃ (path' : Path p m n), path'.Acyclic ∧ ∀ l ∈ path', l ∈ path :=
+theorem Path.exists_acyclic {r : Rel} {m n : Nat} (path : Path r m n) :
+    ∃ (path' : Path r m n), path'.Acyclic ∧ ∀ l ∈ path', l ∈ path :=
   exists_acyclic.aux (Nat.le_refl _)
 
-theorem Program.pathWithout_iff {p : Program} {m n k : Nat} (hk : k < p.size) :
-    m ⟶[p, n]* k ↔ ∃ path : Path p m k, n ∉ path := by
+theorem Program.pathWithout_iff {p : Program} {m n k : Nat} :
+    m ⟶[p, n]* k ↔ ∃ path : Path p.Succ m k, n ∉ path := by
   constructor
   · intro h
     induction h with
     | refl m hne =>
-      exists .refl _ hk
+      exists .refl _
       grind
     | step m l k hne hs h ih =>
-      obtain ⟨path, hn⟩ := ih hk
+      obtain ⟨path, hn⟩ := ih
       exists .step _ _ _ hs path
       grind
   · rintro ⟨path, h⟩
     induction path with grind [intro PathWithout]
 
+theorem Program.bounded_path_succ {p : Program} {m n : Nat}
+    {path : Path p.Succ m n} (hn : n < p.size) : path.Bounded p.size := by
+  intro l hl
+  induction hl with
+  | head n path =>
+    cases path with
+    | refl _ => exact hn
+    | step _ k n hs path => exact hs.1
+  | tail m k n hs path hl ih => exact ih hn
+
 theorem Expr.free_iff' {p : Program} {e : Expr} {n : Nat} :
     e.Free p n ↔
-      e.LocalVar n ∨ ∃ (m k : Nat) (path : Path p m k),
-        e.LocalFn m ∧ (p.fn[k]'path.lt_size_right).LocalVar n ∧ n ∉ path ∧
+      e.LocalVar n ∨ ∃ (m k : Nat) (hk : k < p.size) (path : Path p.Succ m k),
+        e.LocalFn m ∧ p.fn[k].LocalVar n ∧ n ∉ path ∧
         path.length < p.size := by
   constructor
   · intro hf
     obtain hlv | ⟨m, k, hk, hlf, hpath, hlv⟩ := free_iff.mp hf
     · exact .inl hlv
-    · obtain ⟨path, hn⟩ := (Program.pathWithout_iff hk).mp hpath
+    · obtain ⟨path, hn⟩ := Program.pathWithout_iff.mp hpath
       obtain ⟨path', ha, h⟩ := path.exists_acyclic
-      have hlen := Path.length_lt_size_of_acyclic ha
-      exact .inr ⟨m, k, path', hlf, hlv, fun hn' => hn (h _ hn'), hlen⟩
-  · rintro (hlv | ⟨m, k, path, hlf, hlv, hn, hlen⟩)
+      have hlen :=
+        Path.length_lt_size_of_acyclic ha (Program.bounded_path_succ hk)
+      exact .inr ⟨m, k, hk, path', hlf, hlv, fun hn' => hn (h _ hn'), hlen⟩
+  · rintro (hlv | ⟨m, k, hk, path, hlf, hlv, hn, hlen⟩)
     · exact free_of_localVar hlv
-    · have hk := path.lt_size_right
-      have hpath := (Program.pathWithout_iff hk).mpr ⟨path, hn⟩
+    · have hpath := Program.pathWithout_iff.mpr ⟨path, hn⟩
       exact free_iff.mpr <| .inr ⟨m, k, hk, hlf, hpath, hlv⟩
+
+def Program.FnFree (p : Program) (m n : Nat) : Prop :=
+  ∃ hm, n < p.size ∧ n ≠ m ∧ (p.fn[m]'hm).Free p n
+
+theorem Program.bounded_path_fnFree {p : Program} {m n : Nat}
+    {path : Path p.FnFree m n} (hn : n < p.size) : path.Bounded p.size := by
+  intro l hl
+  induction path with
+  | refl n => simp_all
+  | step m k n hs path ih =>
+    obtain ⟨hm, hk, hne, hf⟩ := hs
+    cases hl with
+    | head _ _ => exact hm
+    | tail _ _ _ hs _ hl => exact ih hn hl
+
+theorem Program.nestsEq_iff_exists_path {p : Program} {n m : Nat} :
+      n ≽[p] m ↔ n < p.size ∧ ∃ path : Path p.FnFree m n, path.length < p.size := by
+  suffices n ≽[p] m ↔ n < p.size ∧ ∃ path : Path p.FnFree m n, True by
+    rw [this]
+    constructor <;> rintro ⟨hn, path, -⟩
+    · obtain ⟨path', ha, h⟩ := path.exists_acyclic
+      exact ⟨hn, path',
+        Path.length_lt_size_of_acyclic ha (bounded_path_fnFree hn)⟩
+    · exact ⟨hn, path, .intro⟩
+  constructor
+  · intro h
+    cases h with
+    | refl hn => exact ⟨hn, .refl _, .intro⟩
+    | nests _ h =>
+      induction h with
+      | free n m hn hm hne hf =>
+        exact ⟨hn, .step _ _ _ ⟨hm, hn, hne, hf⟩ (.refl _), by grind⟩
+      | trans n k m h₁ h₂ ih₁ ih₂ =>
+        obtain ⟨hn, path₁, -⟩ := ih₁
+        obtain ⟨hk, path₂, -⟩ := ih₂
+        exact ⟨hn, path₂.concat path₁, .intro⟩
+  · rintro ⟨hn, path, -⟩
+    induction path with
+    | refl n => exact .refl hn
+    | step m k n hs path ih =>
+      obtain ⟨hm, hk, hkm, hf⟩ := hs
+      have h := Nests.free _ _ hk hm hkm hf
+      cases ih hn with
+      | refl hk => exact .nests _ h
+      | nests _ h' =>
+        exact .nests _ (.trans _ _ _ h' h)
 
 def flatMap (s : Std.HashSet Nat) (f : Nat → Std.HashSet Nat) : Std.HashSet Nat :=
   aux ∅ s.toList
@@ -409,15 +481,15 @@ theorem Program.fnFreeVars_correct {p : Program} {m n : Nat} (hm : m < p.size) :
   have hlfs : ∀ {i} (hi : i < p.size) k, k ∈ lfs[i] ↔ p.fn[i].LocalFn k := by
     grind [Expr.fn_in_locals_iff]
   suffices ∀ v i, n ∈ (fnFreeVars.aux p lfs v i)[m]'hm ↔
-      n ∈ v[m] ∨ ∃ (k l : Nat) (path : Path p k l), p.fn[m].LocalFn k ∧
-        n ∈ v[l]'path.lt_size_right ∧ n ∉ path ∧ path.length < i by
+      n ∈ v[m] ∨ ∃ (k l : Nat) (hl : l < p.size) (path : Path p.Succ k l),
+        p.fn[m].LocalFn k ∧ n ∈ v[l] ∧ n ∉ path ∧ path.length < i by
     have := this lvs p.size
     unfold fnFreeVars
     rw [hlc, this]
     simp only [hlvs, Expr.free_iff']
   intro v i
   induction i generalizing v with
-  | zero => grind [fnFreeVars.aux]
+  | zero => simp [fnFreeVars.aux]
   | succ i ih =>
     let update free lf :=
       free ∪ flatMap lf fun m =>
@@ -425,7 +497,7 @@ theorem Program.fnFreeVars_correct {p : Program} {m n : Nat} (hm : m < p.size) :
     specialize ih (v.zipWith update lfs)
     constructor
     · intro h
-      obtain hn | ⟨k, l, path, hlf, hn, hmem, hlen⟩ := ih.mp h <;>
+      obtain hn | ⟨k, l, hl, path, hlf, hn, hmem, hlen⟩ := ih.mp h <;>
         simp only [Vector.getElem_zipWith, mem_union_iff, mem_flatMap_iff, update] at hn
       · obtain hn | ⟨k, hlf, hn⟩ := hn
         · exact .inl hn
@@ -433,24 +505,23 @@ theorem Program.fnFreeVars_correct {p : Program} {m n : Nat} (hm : m < p.size) :
           have hk : k < p.size := by grind
           simp only [hk, ↓reduceDIte, Std.HashSet.mem_erase, beq_eq_false_iff_ne, ne_eq] at hn
           obtain ⟨hne, hn⟩ := hn
-          exact .inr <| ⟨_, _, .refl _ hk, hlf, hn, by grind⟩
+          exact .inr <| ⟨_, _, hk, .refl _, hlf, hn, by grind⟩
       · obtain hn | ⟨o, hlf', hn⟩ := hn
-        · exact .inr ⟨_, _, path, hlf, hn, hmem, by lia⟩
+        · exact .inr ⟨_, _, hl, path, hlf, hn, hmem, by lia⟩
         · rw [hlfs] at hlf'
-          have hl := path.lt_size_right
           have ho : o < p.size := by grind
           simp only [ho, ↓reduceDIte, Std.HashSet.mem_erase, beq_eq_false_iff_ne, ne_eq] at hn
           obtain ⟨hne, hn⟩ := hn
-          exact .inr <| ⟨_, _, path.push ho ⟨hl, hlf'⟩, hlf, hn, by grind⟩
-    · rintro (hn | ⟨k, l, path, hlf, hn, hmem, hlen⟩)
-      · simp [fnFreeVars.aux, update, *]
-      · have hl := path.lt_size_right
-        obtain h | ⟨o, ho, hs, path, rfl⟩ := path.split_last
-        · grind [fnFreeVars.aux]
+          exact .inr <| ⟨_, _, ho, path.push ⟨hl, hlf'⟩, hlf, hn, by grind⟩
+    · erw [ih]
+      rintro (hn | ⟨k, l, hl, path, hlf, hn, hmem, hlen⟩)
+      · simp [update, hn]
+      · obtain h | ⟨o, hs, path, rfl⟩ := path.split_last
+        · grind
         · simp only [Path.length_push, Nat.add_lt_add_iff_right] at hlen
-          have ho := path.lt_size_right
+          have ho := hs.1
           have hn' : n ∈ (v.zipWith update lfs)[o] := by grind [Succ]
-          exact ih.mpr <| .inr ⟨_, _, path, hlf, hn', by grind, hlen⟩
+          exact .inr ⟨_, _, ho, path, hlf, hn', by grind, hlen⟩
 
 def Expr.freeVars (e : Expr) (p : Program) :=
   let (lv, lf) := e.locals
@@ -494,5 +565,102 @@ instance {c : Computation} {n : Nat} : Decidable (c.Free n) :=
 
 instance {c : Computation} : Decidable c.Closed :=
   inferInstanceAs (Decidable (c.expr.Closed c.toProgram))
+
+def Program.nesters (p : Program) : Vector (Std.HashSet Nat) p.size :=
+  let fvs := p.fnFreeVars.mapIdx fun i v => (v.erase i).filter (· < p.size)
+  aux fvs fvs (p.size - 1)
+  where
+    aux fvs v : Nat → _
+      | 0 => v
+      | n + 1 =>
+        let update free fv :=
+          free ∪ flatMap fv fun m =>
+            if hm : m < p.size then v[m] else ∅
+        aux fvs (v.zipWith update fvs) n
+
+theorem Program.nesters_correct {p : Program} {m n : Nat} (hm : m < p.size) :
+    n ∈ p.nesters[m] ↔ n ≻[p] m := by
+  let fvs := p.fnFreeVars.mapIdx fun i v => (v.erase i).filter (· < p.size)
+  have hfvs : ∀ {i} (hi : i < p.size) k, k ∈ fvs[i] ↔ k < p.size ∧ k ≠ i ∧ p.fn[i].Free p k := by
+    grind [fnFreeVars_correct]
+  suffices ∀ v i, (∀ (k : Nat) hk, n ∈ v[k]'hk → n < p.size) →
+    (n ∈ (nesters.aux p fvs v i)[m]'hm ↔
+      n < p.size ∧ (n ∈ v[m] ∨ ∃ (k : Nat) (hk : k < p.size) (path : Path p.FnFree m k),
+        n ∈ v[k] ∧ path.length ≤ i)) by
+    have := this fvs (p.size - 1) (by grind)
+    unfold nesters
+    rw [this]
+    simp only [hfvs]
+    constructor
+    · rintro ⟨hn, ⟨hk, hne, hf⟩ | ⟨k, hk, path, ⟨hn, hne, hf⟩, hlen⟩⟩
+      · exact .free _ _ hn hm hne hf
+      · have h := nestsEq_iff_exists_path.mpr ⟨hk, path, by grind⟩
+        exact nests_iff'.mpr ⟨_, _, hn, hne, hf, h⟩
+    · intro h
+      obtain ⟨k, hk, hn, hne, hf, h⟩ := nests_iff'.mp h
+      obtain ⟨-, path, hlen⟩ := nestsEq_iff_exists_path.mp h
+      exact ⟨hn, .inr ⟨_, hk, path, ⟨hn, hne, hf⟩, by grind⟩⟩
+  intro v i
+  induction i generalizing v with
+  | zero =>
+    intro himp
+    constructor
+    · intro hv
+      simp only [nesters.aux] at hv
+      exact ⟨himp _ hm hv, .inl hv⟩
+    · rintro ⟨hn, hv | ⟨k, hk, path, hv, hlen⟩⟩
+      · simpa [nesters.aux] using hv
+      · simp only [Nat.le_zero_eq, Path.length_eq_zero_iff] at hlen
+        obtain ⟨rfl, rfl⟩ := hlen
+        simpa [nesters.aux] using hv
+  | succ i ih =>
+    let update free fv :=
+      free ∪ flatMap fv fun m =>
+        if hm : m < p.size then v[m] else ∅
+    intro himp
+    replace himp : ∀ (k : Nat) hk, n ∈ (v.zipWith update fvs)[k]'hk → n < p.size := by
+      simp only [Vector.getElem_zipWith, mem_union_iff, mem_flatMap_iff, update]
+      rintro k hk (hv | ⟨l, hf, hv⟩)
+      · exact himp _ hk hv
+      · have hl : l < p.size := by grind
+        simp only [hl, ↓reduceDIte] at hv
+        exact himp _ hl hv
+    specialize ih (v.zipWith update fvs) himp
+    constructor
+    · intro h
+      obtain ⟨hn, hv | ⟨k, hk, path, hv, hlen⟩⟩ := ih.mp h <;>
+        simp only [Vector.getElem_zipWith, mem_union_iff, mem_flatMap_iff, update] at hv
+      · obtain hv | ⟨k, hf, hv⟩ := hv
+        · exact ⟨hn, .inl hv⟩
+        · rw [hfvs] at hf
+          obtain ⟨hk, hne, hf⟩ := hf
+          simp only [hk, ↓reduceDIte] at hv
+          exact ⟨hn, .inr <| ⟨_, hk, .step _ _ _ ⟨hm, hk, hne, hf⟩ (.refl _), hv, by grind⟩⟩
+      · obtain hv | ⟨l, hf, hv⟩ := hv
+        · exact ⟨hn, .inr ⟨_, hk, path, hv, by lia⟩⟩
+        · rw [hfvs] at hf
+          obtain ⟨hl, hne, hf⟩ := hf
+          simp only [hl, ↓reduceDIte] at hv
+          exact ⟨hn, .inr ⟨_, hl, path.push ⟨hk, hl, hne, hf⟩, hv, by grind⟩⟩
+    · erw [ih]
+      rintro ⟨hn, hv | ⟨k, hk, path, hv, hlen⟩⟩
+      · exact ⟨hn, .inl (by simp [update, hv])⟩
+      · obtain ⟨rfl, rfl⟩ | ⟨l, hs, path, rfl⟩ := path.split_last
+        · exact ⟨hn, .inl (by simp [update, hv])⟩
+        · simp only [Path.length_push, Nat.add_le_add_iff_right] at hlen
+          obtain ⟨hl, hk, hne, hf⟩ := hs
+          replace hv : n ∈ (v.zipWith update fvs)[l] := by grind
+          exact ⟨hn, .inr ⟨_, hl, path, hv, hlen⟩⟩
+
+instance {p : Program} {n m : Nat} : Decidable (n ≻[p] m) :=
+  decidable_of_iff (∃ hm : m < p.size, p.nesters[m].contains n) <| by
+    grind [Program.nesters_correct]
+
+instance {p : Program} {n m : Nat} : Decidable (n ≽[p] m) :=
+  decidable_of_iff (∃ hm : m < p.size, n = m ∨ n ≻[p] m) <| by
+    grind [Program.NestsEq]
+
+instance {p : Program} : Decidable p.WF :=
+  decidable_of_iff (∀ n < p.size, n ⊁[p] n) <| by grind [Program.WF]
 
 end
